Uppaal_Networks/UPPAAL_Asm_AbsInt_State_Dumb.thy
@@ -24,17 +24,61 @@ type_synonym dumb = "dumb_base option"
 fun \<gamma>_dumb :: "dumb \<Rightarrow> collect_state set" where
   "\<gamma>_dumb v  = \<gamma>_option (\<lambda>_. \<top>) v"
 
-fun dumb_step :: "dumb astep" where
-  "dumb_step _ _ None _ = None" |
-  "dumb_step (JMPZ target) ipc ins pc = (if pc = Suc ipc \<or> pc = target then Some Any else None)" |
-  "dumb_step CALL ipc ins pc = Some Any" |
-  "dumb_step RETURN ipc ins pc = Some Any" |
-  "dumb_step HALT ipc ins pc = None" |
-  "dumb_step _ ipc ins pc = (if pc = Suc ipc then Some Any else None)"
+fun dumb_steps :: "instr \<Rightarrow> addr \<Rightarrow> dumb \<Rightarrow> (addr * dumb) set" where
+  "dumb_steps _ _ None = {}" |
+  "dumb_steps (JMPZ target) ipc ins = {(target, Some Any), (Suc ipc, Some Any)}" |
+  "dumb_steps CALL ipc ins = \<top>" |
+  "dumb_steps RETURN ipc ins = \<top>" |
+  "dumb_steps HALT ipc ins = {}" |
+  "dumb_steps _ ipc ins = {(Suc ipc, Some Any)}"
+
+definition "dumb_step \<equiv> unique_astep dumb_steps"
+declare dumb_step_def[simp]
+
+fun dumb_step_direct :: "dumb astep" where
+  "dumb_step_direct _ _ None _ = None" |
+  "dumb_step_direct (JMPZ target) ipc ins pc = (if pc = Suc ipc \<or> pc = target then Some Any else None)" |
+  "dumb_step_direct CALL ipc ins pc = Some Any" |
+  "dumb_step_direct RETURN ipc ins pc = Some Any" |
+  "dumb_step_direct HALT ipc ins pc = None" |
+  "dumb_step_direct _ ipc ins pc = (if pc = Suc ipc then Some Any else None)"
+
+lemma dumb_step_direct_eq: "dumb_step = dumb_step_direct"
+proof -
+  have "dumb_step op ipc ins pc = dumb_step_direct op ipc ins pc" for op ipc ins pc
+  proof(cases ins)
+    case (Some a)
+    then show ?thesis
+    proof(cases op)
+      case (JMPZ target)
+      then show ?thesis
+      proof(cases "pc = Suc ipc \<or> pc = target")
+        case True
+        then have "\<forall>sst. (pc, sst) \<in> dumb_steps op ipc ins \<longrightarrow> sst = Some Any" using JMPZ Some by auto
+        then have "dumb_step op ipc ins pc = Some Any" using unique_astep_unique JMPZ Some True dumb_steps.simps(2)
+          by (smt dumb_step_def insertI1 insert_commute)
+        then show ?thesis by (simp add: JMPZ Some True)
+      next
+        case False
+        then have "\<forall>sst. (pc, sst) \<in> dumb_steps op ipc ins \<longrightarrow> sst = None" using JMPZ Some by auto
+        then have "dumb_step op ipc ins pc = None" using unique_astep_unique
+          by (smt CollectD Sup_bot_conv(1) bot_option_def dumb_step_def unique_astep.simps)
+        from this False show ?thesis by (simp add: JMPZ Some)
+      qed
+    next
+      case CALL
+      from this Some show ?thesis by (simp add: Some top_dumb_base_def top_option_def)
+    next
+      case RETURN
+      from this Some show ?thesis by (simp add: Some top_dumb_base_def top_option_def)
+    qed auto
+  qed simp
+  thus "dumb_step = dumb_step_direct" using ext by blast
+qed
 
 global_interpretation AbsInt
   where \<gamma> = \<gamma>_dumb
-    and ai_step = dumb_step
+    and ai_step = dumb_step_direct
 proof (standard, goal_cases)
   case (1 a b)
   then show ?case
@@ -58,8 +102,8 @@ next
     case (Some a)
     then show ?thesis
     proof(cases op)
-      case (JMPZ target) then show ?thesis by (simp add: Some) next
       case (ADD) then show ?thesis using Some collect_step_succ by fastforce next
+      case (JMPZ target) then show ?thesis by (simp add: Some) next
       case (NOT) then show ?thesis using Some collect_step_succ by fastforce next
       case (AND) then show ?thesis using Some collect_step_succ by fastforce next
       case (LT) then show ?thesis using Some collect_step_succ by fastforce next
@@ -74,6 +118,6 @@ next
       case (STOREC c d) then show ?thesis using Some collect_step_succ by simp
     qed auto
   qed
-qed
+qed simp
 
 end
